ModularEngine/src/LogicEngine.FStar/clinical_trials.fst
@@ -209,10 +209,10 @@ let _ =
   let site_recv, send_to_site = createComm portNum_site in
   let phys_recv, send_to_phys = createComm portNum_phys in
   let keyMgr_recv, send_to_keyMgr = createComm portNum_keyMgr in
-  (suscribe [(org, org_recv, send_to_org);
-            (site, site_recv, send_to_site);
-            (phys, phys_recv, send_to_phys);
-            (keyMgr, keyMgr_recv, send_to_keyMgr)];
+  (subscribe [(org, org_recv, send_to_org);
+              (site, site_recv, send_to_site);
+              (phys, phys_recv, send_to_phys);
+              (keyMgr, keyMgr_recv, send_to_keyMgr)];
   Keys.addKey org;
   Keys.addKey site;
   Keys.addKey phys;
